\exercises

\exercise 
Exhibit in tabular form: 
\begin{itemize}
    \item[(a)] 
        $A = \{a : a \in \mathbb{N}, 2 < a < 6\}$
    \item[(b)] 
        $B = \{p : p \in \mathbb{N}, p < 10, p \text{ is odd}\}$
    \item[(c)] 
        $C = \{x : x \in \mathbb{Z}, 2x^2 + x - 6 = 0\}$
\end{itemize}

\answer
\begin{itemize}
    \item[(a)] 
        $A = \{3, 4, 5\}$
    \item[(b)] 
        $B = \{9, 7, 5, 3, 1\}$
    \item[(c)] 
        $C = \{-2\}$
\end{itemize}


\exercise 
Let $A = \{a,b,c,d\}$, $B = \{a,c,g\}$, $C = \{c,g,m,n,p\}$. Then $A \cup B = \{a,b,c,d,g\}$, $A \cup C = \{a,b,c,d,g,m,n,p\}$, $B \cup C = \{a,c,g,m,n,p\}$;

\answer 
\large\textbf{WHAT IS THE QUESTION?}\normalsize


\exercise 
Consider the subsets $K = \{2,4,6,8\}$, $L=\{1,2,3,4\}$, $M=\{3,4,5,6,8\}$ of $U = \{1,2,3,\ldots,10\}$.
\begin{itemize}
    \item[(a)]
        Exhibit $K'$, $L'$, $M'$ in tabular form.
    \item[(b)]
        Show that $(K \cup L)' = K' \cap L'$
\end{itemize}

\answer
\begin{itemize}
    \item[(a)]
        $K' = \{1,3,5,7,9,10\}$ \\
        $L' = \{5,6,7,8,9,10\}$ \\
        $U' = \{1,2,7,9,10\}$
    \item[(b)]
        $K \cup L = \{1,2,3,4,6,8\}$, so $(K \cup L)' = \{5,7,9,10\}$. Using the above, $K' \cap L' = \{5,7,9,10\}$.
\end{itemize}


\exercise \\
\exercise \\
\exercise \\
\exercise


\exercise 
Prove $(A \cup B) \cup C = A \cup (B \cup C)$

\answer 
Any element $x$ belongs to the left hand side if $(x \in A \vee x \in B) \vee x \in C$. It belongs to the right hand side if $x \in A \vee (x \in B \vee x \in C)$. Both expressions are logically equivalent.


\exercise
Prove $(A \cap B) \cap C = A \cap (B \cap C)$

\answer 
Similar answer as the previous-- follows from the associativity of $\wedge$


\exercise
Prove $A \cap (B \cup C) = (A \cap B) \cup (A \cap C)$

\answer
Follows from $\wedge$ distributing over $\vee$


\exercise
Prove $(A \cap B)' = A' \cap B'$

\answer
Follows from DeMorgan's laws


\exercise
Prove $A \cup (B \cap C) = (A \cup B) \cap (A \cup C)$

\answer
Follows from $\vee$ distributing over $\wedge$


\exercise
Prove $A - (B \cup C) = (A - B) \cap (A - C)$

\answer
Follows again from DeMorgan's laws
